Close to being able to extract iostream stuff

core/Combinators.v
@@ -2,13 +2,11 @@ Require Import List.
 Import ListNotations.
 Require Vector String.
 
-Require Import Cheerios.Core.
 Require Import Cheerios.BasicSerializers.
 Require Import Cheerios.DeserializerMonad.
-Import DeserializerNotations.
-Require Import Cheerios.Tactics.
 
-Import ByteListSerializer.
+Require Import Cheerios.Tactics.
+Require Import Cheerios.Types.
 
 (* These functions are either missing obvious implicits, or have
    implicit arguments that are not marked "maximally inserted", which
@@ -19,275 +17,308 @@ Arguments option_map {_ _} _ _.
 Arguments Vector.nil {_}.
 Arguments Vector.cons {_} _ {_} _.
 
+Module Type COMBINATORS (Writer : WRITER) (Reader : READER).
+  Module RWBasic := BasicSerializers Writer Reader.
 
-Section combinators.
+  Parameter list_Serializer : forall A : Type,
+      RWBasic.RWClass.Serializer A -> RWBasic.RWClass.Serializer (list A).
+  Parameter string_Serializer : RWBasic.RWClass.Serializer (String.string).
+End COMBINATORS.
 
+Module Combinators (Writer : WRITER) (Reader : READER) :
+  COMBINATORS Writer Reader.
   (* This section gives instances for various type constructors, including pairs
     and lists. *)
-  Variables A B : Type.
-  Variable sA : Serializer A.
-  Variable sB : Serializer B.
-
-  Definition option_serialize (x : option A) : Serializer.t :=
-    match x with
-    | Some a => Serializer.append (serialize true) (serialize a)
-    | None => serialize false
-    end.
-
-  Definition option_deserialize : Deserializer.t (option A) :=
-    b <- deserialize ;;
-    match b with
-    | true => Some <$> deserialize
-    | false => Deserializer.ret None
-    end.
+  Module RWClass := SerializerClass Writer Reader.
+  Module WRewrite := WriterRewrite Writer.
+  Module RRewrite := ReaderRewrite Reader.
+  Module DeserializerMonad := DeserializerMonad Reader.
+  Module RWBasic := BasicSerializers Writer Reader.
   
-  Lemma option_serialize_deserialize_id :
-    serialize_deserialize_id_spec option_serialize option_deserialize.
-  Proof.
-    intros.
-    unfold option_serialize, option_deserialize.
-    destruct a;
-      repeat (cheerios_crush; simpl).
-  Qed.
+  Import WRewrite.
+  Import RRewrite.
+  Import DeserializerMonad.DeserializerNotations.
+  Import RWBasic.RWClass.
 
-  Global Instance option_Serializer : Serializer (option A).
-  Proof.
-    exact {| serialize := option_serialize;
-             deserialize := option_deserialize;
-             serialize_deserialize_id := option_serialize_deserialize_id |}.
-  Qed.
+  Section BasicCombinators.
+    Variables A B : Type.
+    Variable sA : Serializer A.
+    Variable sB : Serializer B.
 
-  
-  Definition pair_serialize (x : A * B) : Serializer.t :=
-    let (a, b) := x in Serializer.append (serialize a) (serialize b).
-  
-  Definition pair_deserialize : Deserializer.t (A * B) :=
-    Deserializer.bind deserialize
-                      (fun (a : A) =>
-                         Deserializer.bind deserialize
-                                           (fun b =>
-                                              Deserializer.ret (a, b))).
+    Definition bool_Serializer : Serializer bool :=
+      RWBasic.bool_Serializer.
+    
+    Definition option_serialize (x : option A) : Writer.t :=
+      match x with
+      | Some a => Writer.append (fun _ => (serialize true))
+                                (fun _ => (serialize a))
+      | None => serialize false
+      end.
 
-  Lemma pair_serialize_deserialize_id :
-    serialize_deserialize_id_spec pair_serialize pair_deserialize.
-  Proof.
-    intros.
-    unfold pair_serialize, pair_deserialize.
-    destruct a.
-    cheerios_crush.
-  Qed.
+    Definition option_deserialize : Reader.t (option A) :=
+      b <- deserialize ;;
+        match b with
+        | true => Some <$> deserialize
+        | false => Reader.ret None
+        end.
 
-  Global Instance pair_Serializer : Serializer (A * B).
-  Proof.
-    exact {| serialize := pair_serialize;
-             deserialize := pair_deserialize;
-             serialize_deserialize_id := pair_serialize_deserialize_id |}.
-  Qed.
+    Lemma option_serialize_deserialize_id :
+      serialize_deserialize_id_spec option_serialize option_deserialize.
+    Proof.
+      intros.
+      unfold option_serialize, option_deserialize.
+      destruct a;
+        repeat (cheerios_crush; simpl).
+    Qed.
 
-  Definition sum_serialize (x : A + B) : Serializer.t :=
-    match x with
-    | inl a => Serializer.append (serialize true) (serialize a)
-    | inr b => Serializer.append (serialize false) (serialize b)
-    end.
+    Global Instance option_Serializer : Serializer (option A).
+    Proof.
+      exact {| serialize := option_serialize;
+               deserialize := option_deserialize;
+               serialize_deserialize_id := option_serialize_deserialize_id |}.
+    Qed.
 
-  Definition sum_deserialize : Deserializer.t (A + B) :=
-    b <- deserialize ;;
-    match b with
-    | true => inl <$> deserialize
-    | false => inr <$> deserialize
-    end.
+    
+    Definition pair_serialize (x : A * B) : Writer.t :=
+      let (a, b) := x in Writer.append (fun _ => (serialize a))
+                                       (fun _ => (serialize b)).
+    
+    Definition pair_deserialize : Reader.t (A * B) :=
+      Reader.bind deserialize
+                  (fun (a : A) =>
+                     Reader.bind deserialize
+                                 (fun b =>
+                                    Reader.ret (a, b))).
 
-  Lemma sum_serialize_deserialize_id :
-    serialize_deserialize_id_spec sum_serialize sum_deserialize.
-  Proof.
-    unfold sum_serialize, sum_deserialize.
-    destruct a; cheerios_crush.
-  Qed.
-
-  Global Instance sum_Serializer : Serializer (A + B).
-  Proof.
-    exact {| serialize := sum_serialize;
-             deserialize := sum_deserialize;
-             serialize_deserialize_id := sum_serialize_deserialize_id
-          |}.
-  Qed.
-  
-  Fixpoint list_serialize_rec (l : list A) : Serializer.t :=
-    match l with
-    | [] => Serializer.empty
-    | a :: l' => Serializer.append (serialize a) (list_serialize_rec l')
-    end.
-
-  Fixpoint list_serialize_aux (l : list A) (acc : Serializer.t) : Serializer.t :=
-    match l with
-    | [] => acc
-    | a :: l' =>  list_serialize_aux l' (Serializer.append acc (serialize a))
-    end.
-
-  Lemma list_serialize_rec'_aux : forall l acc,
-      Serializer.unwrap (list_serialize_aux l acc) =
-      Serializer.unwrap (Serializer.append acc (list_serialize_rec l)).
-  Proof.
-    intros l.
-    induction l; intros.
-    - simpl.
+    Lemma pair_serialize_deserialize_id :
+      serialize_deserialize_id_spec pair_serialize pair_deserialize.
+    Proof.
+      intros.
+      unfold pair_serialize, pair_deserialize.
+      destruct a.
       cheerios_crush.
-      now rewrite app_nil_r.
-    - unfold list_serialize_aux. fold list_serialize_aux.
+    Qed.
+
+    Global Instance pair_Serializer : Serializer (A * B).
+    Proof.
+      exact {| serialize := pair_serialize;
+               deserialize := pair_deserialize;
+               serialize_deserialize_id := pair_serialize_deserialize_id |}.
+    Qed.
+
+    Definition sum_serialize (x : A + B) : Writer.t :=
+      match x with
+      | inl a => Writer.append (fun _ => (serialize true))
+                               (fun _ => (serialize a))
+      | inr b => Writer.append (fun _ => (serialize false))
+                               (fun _ => (serialize b))
+      end.
+
+    Definition sum_deserialize : Reader.t (A + B) :=
+      b <- deserialize ;;
+        match b with
+        | true => inl <$> deserialize
+        | false => inr <$> deserialize
+        end.
+
+    Lemma sum_serialize_deserialize_id :
+      serialize_deserialize_id_spec sum_serialize sum_deserialize.
+    Proof.
+      unfold sum_serialize, sum_deserialize.
+      destruct a; cheerios_crush.
+    Qed.
+
+    Global Instance sum_Serializer : Serializer (A + B).
+    Proof.
+      exact {| serialize := sum_serialize;
+               deserialize := sum_deserialize;
+               serialize_deserialize_id := sum_serialize_deserialize_id
+            |}.
+    Qed.
+    
+    Fixpoint list_serialize_rec (l : list A) : Writer.t :=
+      match l with
+      | [] => Writer.empty
+      | a :: l' => Writer.append (fun _ => (serialize a))
+                                 (fun _ => (list_serialize_rec l'))
+      end.
+
+    Fixpoint list_serialize_aux (l : list A) (acc : Writer.t) : Writer.t :=
+      match l with
+      | [] => acc
+      | a :: l' =>  list_serialize_aux l' (Writer.append (fun _ => acc)
+                                                         (fun _ => (serialize a)))
+      end.
+
+    Lemma list_serialize_rec'_aux : forall l acc,
+        Writer.unwrap (list_serialize_aux l acc) =
+        Writer.unwrap (Writer.append (fun _ => acc)
+                                     (fun _ => (list_serialize_rec l))).
+    Proof.
+      intros l.
+      induction l; intros.
+      - simpl.
+        cheerios_crush.
+        now rewrite app_nil_r.
+      - unfold list_serialize_aux. fold list_serialize_aux.
+        rewrite IHl.
+        unfold list_serialize_rec at 2.
+        fold list_serialize_rec.
+        cheerios_crush.
+    Qed.
+
+    Definition list_serialize_rec' (l : list A) : Writer.t :=
+      list_serialize_aux l Writer.empty.
+
+    Definition list_serialize (l : list A) : Writer.t :=
+      Writer.append (fun _ => (serialize (length l)))
+                    (fun _ => (list_serialize_rec l)).
+
+    Definition list_serialize' (l : list A) : Writer.t :=
+        Writer.append (fun _ => (serialize (length l)))
+                      (fun _ => (list_serialize_rec' l)).
+
+    Fixpoint list_deserialize_rec (n : nat) : Reader.t (list A) :=
+      match n with
+      | 0 => Reader.ret []
+      | S n' => cons <$> deserialize <*> list_deserialize_rec n'
+      end.
+
+    Definition list_deserialize : Reader.t (list A) :=
+      deserialize >>= list_deserialize_rec.
+
+    Lemma list_serialize_deserialize_id_rec :
+      forall l bin, Reader.unwrap (list_deserialize_rec (length l))
+                                  (Writer.unwrap (list_serialize_rec l) ++ bin)
+                    = Some(l, bin).
+    Proof.
+      intros.
+      unfold list_serialize_rec.
+      cheerios_crush. simpl.
+      induction l;
+        simpl;
+        cheerios_crush.
+      unfold DeserializerMonad.sequence.
       rewrite IHl.
-      unfold list_serialize_rec at 2.
-      fold list_serialize_rec.
       cheerios_crush.
-  Qed.
+    Qed.
 
-  Definition list_serialize_rec' (l : list A) : Serializer.t :=
-    list_serialize_aux l Serializer.empty.
-
-  Definition list_serialize (l : list A) : Serializer.t :=
-    Serializer.append (serialize (length l)) (list_serialize_rec l).
-
-  Definition list_serialize' (l : list A) : Serializer.t :=
-    Serializer.append (serialize (length l)) (list_serialize_rec' l).
-
-  Fixpoint list_deserialize_rec (n : nat) : Deserializer.t (list A) :=
-    match n with
-    | 0 => Deserializer.ret []
-    | S n' => cons <$> deserialize <*> list_deserialize_rec n'
-    end.
-
-  Definition list_deserialize : Deserializer.t (list A) :=
-    deserialize >>= list_deserialize_rec.
-
-  Lemma list_serialize_deserialize_id_rec :
-    forall l bin, Deserializer.unwrap (list_deserialize_rec (length l))
-                                      (Serializer.unwrap (list_serialize_rec l) ++ bin)
-                  = Some(l, bin).
-  Proof.
-    intros.
-    unfold list_serialize_rec.
-    cheerios_crush. simpl.
-    induction l;
-      simpl;
+    Lemma list_serialize_deserialize_id :
+      serialize_deserialize_id_spec list_serialize list_deserialize.
+    Proof.
+      unfold list_serialize, list_deserialize.
       cheerios_crush.
-    unfold sequence.
-    cheerios_crush. 
-    rewrite IHl.
-    cheerios_crush.
-  Qed.
+      now rewrite list_serialize_deserialize_id_rec.
+    Qed.
 
-  Lemma list_serialize_deserialize_id :
-    serialize_deserialize_id_spec list_serialize list_deserialize.
-  Proof.
-    unfold list_serialize, list_deserialize.
-    cheerios_crush.
-    now rewrite list_serialize_deserialize_id_rec.
-  Qed.
+    Lemma list_serialize'_deserialize_id_rec :
+      forall l bin, Reader.unwrap (list_deserialize_rec (length l))
+                                  (Writer.unwrap (list_serialize_rec' l) ++ bin)
+                    = Some(l, bin).
+    Proof.
+      intros.
+      unfold list_serialize_rec'.
+      rewrite list_serialize_rec'_aux.
+      cheerios_crush. simpl.
+      now rewrite list_serialize_deserialize_id_rec.
+    Qed.
 
-  Lemma list_serialize'_deserialize_id_rec :
-    forall l bin, Deserializer.unwrap (list_deserialize_rec (length l))
-                                      (Serializer.unwrap (list_serialize_rec' l) ++ bin)
-                  = Some(l, bin).
-  Proof.
-    intros.
-    unfold list_serialize_rec'.
-    rewrite list_serialize_rec'_aux.
-    cheerios_crush. simpl.
-    now rewrite list_serialize_deserialize_id_rec.
-  Qed.
-
-  Lemma list_serialize'_deserialize_id :
-    serialize_deserialize_id_spec list_serialize' list_deserialize.
-  Proof.
-    unfold list_serialize', list_deserialize.
-    cheerios_crush.
-    now rewrite list_serialize'_deserialize_id_rec.
-  Qed.
-
-  Global Instance list_Serializer : Serializer (list A).
-  Proof.
-    exact {| serialize := list_serialize';
-             deserialize := list_deserialize;
-             serialize_deserialize_id := list_serialize'_deserialize_id
-          |}.
-  Qed.
-
-  Fixpoint vector_serialize {n} (v : Vector.t A n) : Serializer.t :=
-    match v with
-    | Vector.nil => Serializer.empty
-    | Vector.cons a v' => Serializer.append (serialize a) (vector_serialize v')
-    end.
-
-  Fixpoint vector_deserialize {n} : Deserializer.t (Vector.t A n) :=
-    match n as n0 return Deserializer.t (Vector.t A n0) with
-    | 0 => Deserializer.ret Vector.nil
-    | S n' => a <- deserialize ;;
-                v <- vector_deserialize ;;
-                Deserializer.ret (Vector.cons a v)
-    end.
-
-  Lemma vector_serialize_deserialize_id :
-    forall n, serialize_deserialize_id_spec vector_serialize (@vector_deserialize n).
-  Proof.
-    induction n; intros.
-    - destruct a using Vector.case0. auto. unfold vector_serialize,  vector_deserialize.
+    Lemma list_serialize'_deserialize_id :
+      serialize_deserialize_id_spec list_serialize' list_deserialize.
+    Proof.
+      unfold list_serialize', list_deserialize.
       cheerios_crush.
-    - destruct a using Vector.caseS'.
-      simpl.
-      cheerios_crush.
-      rewrite IHn.
-      cheerios_crush.
-  Qed.
-
-  Global Instance vector_Serializer n : Serializer (Vector.t A n).
-  Proof.
-    exact {| serialize := vector_serialize;
-             deserialize := vector_deserialize;
-             serialize_deserialize_id := vector_serialize_deserialize_id n
-          |}.
-  Qed.
-End combinators.
+      now rewrite list_serialize'_deserialize_id_rec.
+    Qed.
 
 
-(* This has to go here because it depends on having a serializer for
+    Global Instance list_Serializer : Serializer (list A).
+    Proof.
+      exact {| serialize := list_serialize';
+               deserialize := list_deserialize;
+               serialize_deserialize_id := list_serialize'_deserialize_id
+            |}.
+    Qed.
+
+    Fixpoint vector_serialize {n} (v : Vector.t A n) : Writer.t :=
+      match v with
+      | Vector.nil => Writer.empty
+      | Vector.cons a v' => Writer.append (fun _ => (serialize a))
+                                          (fun _ => (vector_serialize v'))
+      end.
+
+    Fixpoint vector_deserialize {n} : Reader.t (Vector.t A n) :=
+      match n as n0 return Reader.t (Vector.t A n0) with
+      | 0 => Reader.ret Vector.nil
+      | S n' => a <- deserialize ;;
+                  v <- vector_deserialize ;;
+                  Reader.ret (Vector.cons a v)
+      end.
+
+    Lemma vector_serialize_deserialize_id :
+      forall n, serialize_deserialize_id_spec vector_serialize (@vector_deserialize n).
+    Proof.
+      induction n; intros.
+      - destruct a using Vector.case0. auto. unfold vector_serialize,  vector_deserialize.
+        cheerios_crush.
+      - destruct a using Vector.caseS'.
+        simpl.
+        cheerios_crush.
+        rewrite IHn.
+        cheerios_crush.
+    Qed.
+
+    Global Instance vector_Serializer n : Serializer (Vector.t A n).
+    Proof.
+      exact {| serialize := vector_serialize;
+               deserialize := vector_deserialize;
+               serialize_deserialize_id := vector_serialize_deserialize_id n
+            |}.
+    Qed.
+  End BasicCombinators.
+
+
+    (* This has to go here because it depends on having a serializer for
    lists available. *)
 
-Fixpoint string_to_list s :=
-  match s with
-  | String.EmptyString => nil
-  | String.String c s' => c :: (string_to_list s')
-  end.
+    Fixpoint string_to_list s :=
+      match s with
+      | String.EmptyString => nil
+      | String.String c s' => c :: (string_to_list s')
+      end.
 
-Fixpoint list_to_string l :=
-  match l with
-  | nil => String.EmptyString
-  | h::l' => String.String h (list_to_string l')
-  end.
+    Fixpoint list_to_string l :=
+      match l with
+      | nil => String.EmptyString
+      | h::l' => String.String h (list_to_string l')
+      end.
 
-Lemma string_to_list_to_string :
-  forall s, list_to_string (string_to_list s) = s.
-Proof.
-  induction s; auto; simpl.
-  now rewrite IHs.
-Qed.
+    Lemma string_to_list_to_string :
+      forall s, list_to_string (string_to_list s) = s.
+    Proof.
+      induction s; auto; simpl.
+      now rewrite IHs.
+    Qed.
 
-Definition string_serialize (s : String.string) :=
-  serialize (string_to_list s).
+    Definition string_serialize (s : String.string) :=
+      serialize (string_to_list s).
 
-Definition string_deserialize : Deserializer.t String.string :=
-  list_to_string <$> deserialize.
+    Definition string_deserialize : Reader.t String.string :=
+      list_to_string <$> deserialize.
 
-Lemma string_serialize_deserialize_id :
-  serialize_deserialize_id_spec string_serialize string_deserialize.
-Proof.
-  unfold string_deserialize, string_serialize.
-  cheerios_crush.
-  now rewrite string_to_list_to_string.
-Qed.
+    Lemma string_serialize_deserialize_id :
+      serialize_deserialize_id_spec string_serialize string_deserialize.
+    Proof.
+      unfold string_deserialize, string_serialize.
+      cheerios_crush.
+      now rewrite string_to_list_to_string.
+    Qed.
 
-Instance string_Serializer : Serializer String.string.
-Proof.
-  exact {| serialize := string_serialize;
-           deserialize := string_deserialize;
-           serialize_deserialize_id := string_serialize_deserialize_id
-        |}.
-Qed.
+    Instance string_Serializer : Serializer String.string.
+    Proof.
+      exact {| serialize := string_serialize;
+               deserialize := string_deserialize;
+               serialize_deserialize_id := string_serialize_deserialize_id
+            |}.
+    Qed.
+End Combinators.
