core/Tree.v
@@ -1,9 +1,8 @@
-Require Import Cheerios.BasicSerializers.
-Require Import Cheerios.Core.
+Require Import Cheerios.Combinators.
 Require Import Cheerios.DeserializerMonad.
+Require Import Cheerios.Tactics.
 Require Import Cheerios.Types.
 
-Import ByteListSerializer.
 (*
    Most user-defined datatypes are tree-like, which are typically nontrivial to
    deserialize by structural recursion on the bitstream. This file provides a
@@ -15,8 +14,6 @@ Require Import List.
 Import ListNotations.
 
 Require Import Cheerios.Cheerios.
-Import DeserializerNotations.
-
 Set Implicit Arguments.
 
 Section tree.
@@ -70,676 +67,706 @@ Section tree.
   End tree_ind.
 End tree.
 
-Fixpoint rev_rec {A} (l : list A) (acc : list A) :=
-  match l with
-  | [] => acc
-  | a :: l => rev_rec l (a :: acc)
-  end.
+Module TreeSerializer (Writer : WRITER) (Reader : READER).
+  Module RWClass := SerializerClass Writer Reader.
+  Module RWCombinators := Combinators Writer Reader.
+  Module DeserializerMonad := DeserializerMonad Reader.
+  Module WRewrite := WriterRewrite Writer.
+  Module RRewrite := ReaderRewrite Reader.
 
-Lemma rev_rec_spec : forall {A : Type} (l : list A) acc,
-    rev_rec l acc = rev l ++ acc.
-Proof.
-  intros A l.
-  induction l.
-  - reflexivity.
-  - intros.
-    simpl.
-    rewrite <- app_assoc.
-    now rewrite IHl.
-Qed.
+  Import DeserializerMonad.DeserializerNotations.
+  Import RWCombinators.RWBasic.
+  Import WRewrite.
+  Import RRewrite.
+  
 
-Definition rev' {A} (l : list A) :=
-  rev_rec l [].
 
-Fixpoint map_rec {A B} (f : A -> B) (l : list A) (acc : list B) :=
-  match l with
-  | [] => rev' acc
-  | a :: l => map_rec f l (f a :: acc)
-  end.
-
-Lemma map_rec_spec : forall {A B} (f : A -> B) (l : list A) (acc : list B),
-    map_rec f l acc = rev acc ++ List.map f l.
-Proof.
-  intros A B f l.
-  induction l.
-  - intros.
-    simpl.
-    unfold rev'.
-    now rewrite rev_rec_spec.
-  - intros.
-    simpl.
-    rewrite IHl.
-    simpl.
-    rewrite <- app_assoc.
-    reflexivity.
-Qed.
-
-Definition list_map' {A B} (f : A -> B) (l : list A) :=
-  map_rec f l [].
-
-Theorem map'_spec : forall {A B} (f : A -> B) (l : list A),
-    List.map f l = list_map' f l.
-  intros.
-  unfold list_map'.
-  now rewrite map_rec_spec.
-Qed.
-
-(* The shape of a tree can be expressed by mapping (fun _ => tt) over it. *)
-Fixpoint map {A B} (f : A -> B) (t : tree A) : tree B :=
-  match t with
-  | atom a => atom (f a)
-  | node l => node (List.map (map f) l)
-  end.
-
-Definition shape {A} (t : tree A) : tree unit :=
-  map (fun _ => tt) t.
-
-Fixpoint tree_map' {A B} (f : A -> B) (t : tree A) : tree B :=
-  let fix tree_map_loop {A B} (f : A -> B) (l : list (tree A)) acc :=
+  Fixpoint rev_rec {A} (l : list A) (acc : list A) :=
     match l with
-    | [] => rev_rec acc []
-    | a :: l => tree_map_loop f l (map f a :: acc)
-    end in
-  match t with
-  | atom a => atom (f a)
-  | node l => node (tree_map_loop f l [])
-  end.
-
-Definition tree_map_loop :=
-  fix tree_map_loop {A B} (f : A -> B) (l : list (tree A)) acc :=
-    match l with
-    | [] => rev_rec acc []
-    | a :: l => tree_map_loop f l (map f a :: acc)
+    | [] => acc
+    | a :: l => rev_rec l (a :: acc)
     end.
 
-Check @map_rec_spec.
-Lemma tree_map_loop_spec :
-      forall {A B} (f : A -> B) l acc,
-        tree_map_loop f l acc = rev acc ++ List.map (map f) l.
-Proof.
-  intros A B f l.
-  induction l; intros.
-  - simpl.
-    now rewrite rev_rec_spec.
-  - simpl.
-    rewrite IHl.
-    simpl.
-    now rewrite <- app_assoc.
-Qed.
+  Lemma rev_rec_spec : forall {A : Type} (l : list A) acc,
+      rev_rec l acc = rev l ++ acc.
+  Proof.
+    intros A l.
+    induction l.
+    - reflexivity.
+    - intros.
+      simpl.
+      rewrite <- app_assoc.
+      now rewrite IHl.
+  Qed.
 
-Theorem tree_map'_spec : forall {A B} (f : A -> B) (t : tree A),
-    tree_map' f t = map f t.
-Proof.
-  intros.
-  destruct t.
-  - reflexivity.
-  - simpl.
-    now rewrite tree_map_loop_spec.
-Qed.
+  Definition rev' {A} (l : list A) :=
+    rev_rec l [].
 
-(* Fill out a tree using a list of elements given in preorder traversal order. *)
-Fixpoint fill' {A B} (x : tree A) (bs : list B) : option (tree B * list B) :=
-  let fix fill'_list (l : list (tree A)) (bs : list B) : option (list (tree B) * list B) :=
-      match l with
-      | [] => Some ([], bs)
-      | x :: l => match fill' x bs with None => None
-                 | Some (x, bs) =>
-                 match fill'_list l bs with None => None
-                 | Some (l, bs) =>
-                 Some (x :: l, bs)
-                 end
-                 end
-      end in
-  match x with
-  | atom _ => match bs with
-             | [] => None
-             | b :: bs => Some (atom b, bs)
-             end
-  | node l => match fill'_list l bs with None => None
-             | Some (l, bs) => Some (node l, bs)
-             end
+  Fixpoint map_rec {A B} (f : A -> B) (l : list A) (acc : list B) :=
+    match l with
+    | [] => rev' acc
+    | a :: l => map_rec f l (f a :: acc)
+    end.
 
-  end.
+  Lemma map_rec_spec : forall {A B} (f : A -> B) (l : list A) (acc : list B),
+      map_rec f l acc = rev acc ++ List.map f l.
+  Proof.
+    intros A B f l.
+    induction l.
+    - intros.
+      simpl.
+      unfold rev'.
+      now rewrite rev_rec_spec.
+    - intros.
+      simpl.
+      rewrite IHl.
+      simpl.
+      rewrite <- app_assoc.
+      reflexivity.
+  Qed.
 
-(* Copy paste of local definition above. *)
-Definition fill'_list {A B} :=
-  fix fill'_list (l : list (tree A)) (bs : list B) : option (list (tree B) * list B) :=
-      match l with
-      | [] => Some ([], bs)
-      | x :: l => match fill' x bs with None => None
-                 | Some (x, bs) =>
-                 match fill'_list l bs with None => None
-                 | Some (l, bs) =>
-                 Some (x :: l, bs)
-                 end
-                 end
-      end.
+  Definition list_map' {A B} (f : A -> B) (l : list A) :=
+    map_rec f l [].
 
-Definition fill {A B} (x : tree A) (bs : list B) : option (tree B) :=
-  match fill' x bs with None => None
-  | Some (t, _) => Some t
-  end.
+  Theorem map'_spec : forall {A B} (f : A -> B) (l : list A),
+      List.map f l = list_map' f l.
+    intros.
+    unfold list_map'.
+    now rewrite map_rec_spec.
+  Qed.
 
-(* Produce a preorder traversal list of elements *)
-Fixpoint preorder {A} (x : tree A) : list A :=
-  let fix preorder_list (l : list (tree A)) : list A :=
-      match l with
-      | [] => []
-      | x :: l => preorder x ++ preorder_list l
-      end
-  in
-  match x with
-  | atom a => [a]
-  | node l => preorder_list l
-  end.
+  (* The shape of a tree can be expressed by mapping (fun _ => tt) over it. *)
+  Fixpoint map {A B} (f : A -> B) (t : tree A) : tree B :=
+    match t with
+    | atom a => atom (f a)
+    | node l => node (List.map (map f) l)
+    end.
 
-Definition preorder_list {A} :=
-  fix preorder_list (l : list (tree A)) : list A :=
-      match l with
-      | [] => []
-      | x :: l => preorder x ++ preorder_list l
-      end.
+  Definition shape {A} (t : tree A) : tree unit :=
+    map (fun _ => tt) t.
 
-Fixpoint preorder' {A} (x : tree A) : list A :=
-  let fix preorder_list (l : list (tree A)) acc : list A :=
-      match l with
-      | [] => acc
-      | x :: l => preorder_list l (acc ++ preorder x)
-      end
-  in
-  match x with
-  | atom a => [a]
-  | node l => preorder_list l []
-  end.
-
-(* Since the shape is expressed as mapping, we will need the fact that filling
-   out the a mapped tree with the elements of the original tree gives the
-   original.
- *)
-Lemma fill'_preorder :
-  forall A B (f : B -> A) t (bs : list B),
-    fill' (map f t) (preorder t ++ bs) = Some (t, bs).
-Proof.
-  intros A B f.
-  induction t using tree_rect
-  with (P_list := fun l =>
-     forall bs,
-       fill'_list (List.map (map f) l) (preorder_list l ++ bs) = Some (l, bs)); intros.
-  - auto.
-  - simpl.
-    rewrite app_ass. rewrite  IHt. rewrite IHt0. auto.
-  - auto.
-  - simpl.
-    fold (@preorder_list B).
-    fold (@fill'_list A B).
-    now rewrite IHt.
-Qed.
-
-Lemma fill_preorder :
-  forall A B (f : A -> B) t,
-    fill (map f t) (preorder t) = Some t.
-Proof.
-  unfold fill.
-  intros.
-  rewrite <- app_nil_r with (l := preorder t).
-  now rewrite fill'_preorder.
-Qed.
-
-Section serializer.
-  Variables A : Type.
-  Variable sA : Serializer A.
-
-  (* Now we're ready to serialize trees. First, we serialize their shape. *)
-
-  Fixpoint serialize_tree_shape (t : tree A) : Serializer.t :=
-    let fix serialize_list_tree_shape (l : list (tree A)) : Serializer.t :=
+  Fixpoint tree_map' {A B} (f : A -> B) (t : tree A) : tree B :=
+    let fix tree_map_loop {A B} (f : A -> B) (l : list (tree A)) acc :=
         match l with
-        | [] => Serializer.empty
-        | x :: xs => Serializer.append (serialize_tree_shape x)
-                                       (serialize_list_tree_shape xs)
+        | [] => rev_rec acc []
+        | a :: l => tree_map_loop f l (map f a :: acc)
         end in
     match t with
-    | atom _ => serialize x00 (* ignore the data, since we're just focused on the shape *)
-    | node l => Serializer.append (serialize x01)
-                                  (Serializer.append
-                                     (serialize_list_tree_shape l)
-                                     (serialize x02))
+    | atom a => atom (f a)
+    | node l => node (tree_map_loop f l [])
     end.
 
-  Fixpoint serialize_tree_shape' (t : tree A) : Serializer.t :=
-    let fix serialize_list_tree_shape (l : list (tree A)) acc : Serializer.t :=
+  Definition tree_map_loop :=
+    fix tree_map_loop {A B} (f : A -> B) (l : list (tree A)) acc :=
+      match l with
+      | [] => rev_rec acc []
+      | a :: l => tree_map_loop f l (map f a :: acc)
+      end.
+
+  Check @map_rec_spec.
+  Lemma tree_map_loop_spec :
+    forall {A B} (f : A -> B) l acc,
+      tree_map_loop f l acc = rev acc ++ List.map (map f) l.
+  Proof.
+    intros A B f l.
+    induction l; intros.
+    - simpl.
+      now rewrite rev_rec_spec.
+    - simpl.
+      rewrite IHl.
+      simpl.
+      now rewrite <- app_assoc.
+  Qed.
+
+  Theorem tree_map'_spec : forall {A B} (f : A -> B) (t : tree A),
+      tree_map' f t = map f t.
+  Proof.
+    intros.
+    destruct t.
+    - reflexivity.
+    - simpl.
+      now rewrite tree_map_loop_spec.
+  Qed.
+
+  (* Fill out a tree using a list of elements given in preorder traversal order. *)
+  Fixpoint fill' {A B} (x : tree A) (bs : list B) : option (tree B * list B) :=
+    let fix fill'_list (l : list (tree A)) (bs : list B) : option (list (tree B) * list B) :=
         match l with
-        | [] => acc
-        | x :: xs =>
-          serialize_list_tree_shape xs
-                                    (Serializer.append acc (serialize_tree_shape x))
+        | [] => Some ([], bs)
+        | x :: l => match fill' x bs with None => None
+                                     | Some (x, bs) =>
+                                       match fill'_list l bs with None => None
+                                                             | Some (l, bs) =>
+                                                               Some (x :: l, bs)
+                                       end
+                    end
+        end in
+    match x with
+    | atom _ => match bs with
+                | [] => None
+                | b :: bs => Some (atom b, bs)
+                end
+    | node l => match fill'_list l bs with None => None
+                                      | Some (l, bs) => Some (node l, bs)
+                end
+
+    end.
+
+  (* Copy paste of local definition above. *)
+  Definition fill'_list {A B} :=
+    fix fill'_list (l : list (tree A)) (bs : list B) : option (list (tree B) * list B) :=
+      match l with
+      | [] => Some ([], bs)
+      | x :: l => match fill' x bs with None => None
+                                   | Some (x, bs) =>
+                                     match fill'_list l bs with None => None
+                                                           | Some (l, bs) =>
+                                                             Some (x :: l, bs)
+                                     end
+                  end
+      end.
+
+  Definition fill {A B} (x : tree A) (bs : list B) : option (tree B) :=
+    match fill' x bs with None => None
+                     | Some (t, _) => Some t
+    end.
+
+  (* Produce a preorder traversal list of elements *)
+  Fixpoint preorder {A} (x : tree A) : list A :=
+    let fix preorder_list (l : list (tree A)) : list A :=
+        match l with
+        | [] => []
+        | x :: l => preorder x ++ preorder_list l
         end
     in
-    match t with
-    | atom _ => serialize x00 (* ignore the data, since we're just focused on the shape *)
-    | node l => Serializer.append (serialize x01)
-                                  (Serializer.append
-                                     (serialize_list_tree_shape l Serializer.empty)
-                                     (serialize x02))
+    match x with
+    | atom a => [a]
+    | node l => preorder_list l
     end.
 
-  Definition serialize_list_tree_shape :=
-    fix serialize_list_tree_shape (l : list (tree A)) : Serializer.t :=
+  Definition preorder_list {A} :=
+    fix preorder_list (l : list (tree A)) : list A :=
+      match l with
+      | [] => []
+      | x :: l => preorder x ++ preorder_list l
+      end.
+
+  Fixpoint preorder' {A} (x : tree A) : list A :=
+    let fix preorder_list (l : list (tree A)) acc : list A :=
         match l with
-        | [] => Serializer.empty
-        | x :: xs => Serializer.append (serialize_tree_shape x)
-                                       (serialize_list_tree_shape xs)
+        | [] => acc
+        | x :: l => preorder_list l (acc ++ preorder x)
+        end
+    in
+    match x with
+    | atom a => [a]
+    | node l => preorder_list l []
+    end.
+
+  (* Since the shape is expressed as mapping, we will need the fact that filling
+   out the a mapped tree with the elements of the original tree gives the
+   original.
+   *)
+  Lemma fill'_preorder :
+    forall A B (f : B -> A) t (bs : list B),
+      fill' (map f t) (preorder t ++ bs) = Some (t, bs).
+  Proof.
+    intros A B f.
+    induction t using tree_rect
+      with (P_list := fun l =>
+                        forall bs,
+                          fill'_list (List.map (map f) l) (preorder_list l ++ bs) = Some (l, bs)); intros.
+    - auto.
+    - simpl.
+      rewrite app_ass. rewrite  IHt. rewrite IHt0. auto.
+    - auto.
+    - simpl.
+      fold (@preorder_list B).
+      fold (@fill'_list A B).
+      now rewrite IHt.
+  Qed.
+
+  Lemma fill_preorder :
+    forall A B (f : A -> B) t,
+      fill (map f t) (preorder t) = Some t.
+  Proof.
+    unfold fill.
+    intros.
+    rewrite <- app_nil_r with (l := preorder t).
+    now rewrite fill'_preorder.
+  Qed.
+
+  Section serializer.
+    Variables A : Type.
+    Variable sA : Serializer A.
+
+    (* Now we're ready to serialize trees. First, we serialize their shape. *)
+
+    Fixpoint serialize_tree_shape (t : tree A) : Writer.t :=
+      let fix serialize_list_tree_shape (l : list (tree A)) : Writer.t :=
+          match l with
+          | [] => Writer.empty
+          | x :: xs => Writer.append (fun _ => (serialize_tree_shape x))
+                                     (fun _ => (serialize_list_tree_shape xs))
+          end in
+      match t with
+      | atom _ => serialize x00 (* ignore the data, since we're just focused on the shape *)
+      | node l => Writer.append (fun _ => (serialize x01))
+                                (fun _ => (Writer.append
+                                             (fun _ => serialize_list_tree_shape l)
+                                             (fun _ => (serialize x02))))
+      end.
+
+    Fixpoint serialize_tree_shape' (t : tree A) : Writer.t :=
+      let fix serialize_list_tree_shape (l : list (tree A)) acc : Writer.t :=
+          match l with
+          | [] => acc
+          | x :: xs =>
+            serialize_list_tree_shape xs
+                                      (Writer.append (fun _ => acc)
+                                                     (fun _ => (serialize_tree_shape x)))
+          end
+      in
+      match t with
+      | atom _ => serialize x00 (* ignore the data, since we're just focused on the shape *)
+      | node l => Writer.append (fun _ => (serialize x01))
+                                (fun _ => (Writer.append
+                                             (fun _ => serialize_list_tree_shape l Writer.empty)
+                                             (fun _ => serialize x02)))
+      end.
+
+    Definition serialize_list_tree_shape :=
+      fix serialize_list_tree_shape (l : list (tree A)) : Writer.t :=
+        match l with
+        | [] => Writer.empty
+        | x :: xs => Writer.append (fun _ => serialize_tree_shape x)
+                                   (fun _ => serialize_list_tree_shape xs)
         end.
 
-  Definition deserialize_tree_shape_step (b : byte) (s : list (list (tree unit))) :
-    fold_state (list (list (tree unit))) (tree unit) :=
-    match b with
-    | x00 => match s with
-             | [] => Done (atom tt)
-             | ts :: s => More ((atom tt :: ts) :: s)
-             end
-    | x01 => More ([] :: s)
-    | x02 => match s with
-             | [] => Error
-             | ts :: s => let t := node (List.rev ts) in
-                          match s with
-                          | [] => Done t
-                          | ts :: acc => More ((t :: ts) :: acc)
-                          end
-             end
+    Definition deserialize_tree_shape_step (b : byte) (s : list (list (tree unit))) :
+      fold_state (list (list (tree unit))) (tree unit) :=
+      match b with
+      | x00 => match s with
+               | [] => Done (atom tt)
+               | ts :: s => More ((atom tt :: ts) :: s)
+               end
+      | x01 => More ([] :: s)
+      | x02 => match s with
+               | [] => Error
+               | ts :: s => let t := node (List.rev ts) in
+                            match s with
+                            | [] => Done t
+                            | ts :: acc => More ((t :: ts) :: acc)
+                            end
+               end
 
-    | _ => Error
-    end.
-
-  Lemma shape_aux :
-    forall t acc bytes,
-      Deserializer.unwrap (Deserializer.fold deserialize_tree_shape_step acc)
-                          (Serializer.unwrap (serialize_tree_shape t) ++ bytes) =
-      match acc with
-      | [] => Some (shape t, bytes)
-      | j :: js => Deserializer.unwrap
-                     (Deserializer.fold deserialize_tree_shape_step
-                                        ((shape t :: j) :: js)) bytes
+      | _ => Error
       end.
-  Proof.
-    induction t using tree_rect with
-        (P_list := fun l =>
-       (* We need to extend the statement to a list of subtrees for the mutual induction
+
+    Lemma shape_aux :
+      forall t acc bytes,
+        Reader.unwrap (Reader.fold deserialize_tree_shape_step acc)
+                      (Writer.unwrap (serialize_tree_shape t) ++ bytes) =
+        match acc with
+        | [] => Some (shape t, bytes)
+        | j :: js => Reader.unwrap
+                       (Reader.fold deserialize_tree_shape_step
+                                    ((shape t :: j) :: js)) bytes
+        end.
+    Proof.
+      induction t using tree_rect with
+          (P_list := fun l =>
+                       (* We need to extend the statement to a list of subtrees for the mutual induction
           hypothesis.
           It says that serializing and then deserializing a list of trees `l` is the same
           as `List.map (map (fun _ => tt) l)`.
           `deserialize_list_tree_shape'` is always called with at least one element on the
           accumulator, so there's no need for a match like there was above.
-        *)
-       forall ts acc bytes,
-         Deserializer.unwrap
-           (Deserializer.fold deserialize_tree_shape_step (ts :: acc))
-           (Serializer.unwrap (serialize_list_tree_shape l) ++ bytes) =
-         Deserializer.unwrap
-           (Deserializer.fold
-              deserialize_tree_shape_step
-              ((List.rev (List.map shape l) ++ ts) :: acc)) bytes);
-      intros;
-      try (unfold serialize_list_tree_shape;
-           rewrite Serializer.append_unwrap, app_ass, IHt, IHt0;
-           simpl;
-           now rewrite app_ass);
-      (cheerios_crush; simpl; cheerios_crush; simpl);
-      destruct acc;
-      auto;
-      rewrite IHt;
-      rewrite Deserializer.fold_unwrap;
-      simpl;
-      now rewrite app_nil_r, rev_involutive.
-  Qed.
-  
-  Definition deserialize_tree_shape : Deserializer.t (tree unit) :=
-    Deserializer.fold deserialize_tree_shape_step [].
+                        *)
+                       forall ts acc bytes,
+                         Reader.unwrap
+                           (Reader.fold deserialize_tree_shape_step (ts :: acc))
+                           (Writer.unwrap (serialize_list_tree_shape l) ++ bytes) =
+                         Reader.unwrap
+                           (Reader.fold
+                              deserialize_tree_shape_step
+                              ((List.rev (List.map shape l) ++ ts) :: acc)) bytes);
+        intros;
+        try (unfold serialize_list_tree_shape;
+             rewrite Writer.append_unwrap, app_ass, IHt, IHt0;
+             simpl;
+             now rewrite app_ass).
+      (cheerios_crush; simpl; cheerios_crush; simpl).
+      - destruct acc;
+          cheerios_crush;
+          simpl;
+          rewrite byte_unwrap;
+          simpl;
+          cheerios_crush.
+      - destruct acc;
+          rewrite Reader.fold_unwrap;
+          simpl; rewrite Writer.append_unwrap;
+            simpl;
+            rewrite byte_unwrap;
+            simpl;
+            rewrite Writer.append_unwrap;
+            fold serialize_list_tree_shape;
+            rewrite app_ass;
+            rewrite IHt;
+            rewrite Reader.fold_unwrap;
+            rewrite byte_unwrap; simpl;
+              now rewrite app_nil_r, rev_involutive. 
+    Qed.
+    
+    Definition deserialize_tree_shape : Reader.t (tree unit) :=
+      Reader.fold deserialize_tree_shape_step [].
 
-  (* This is the top level statement about serializing and deserializing tree shapes:
+    (* This is the top level statement about serializing and deserializing tree shapes:
      it results in `shape` of the original tree. *)
-  Lemma serialize_deserialize_shape_id :
-    forall t bytes,
-      Deserializer.unwrap deserialize_tree_shape
-                          (Serializer.unwrap (serialize_tree_shape t) ++ bytes)
-      = Some (shape t, bytes).
-  Proof.
-    intros.
-    unfold deserialize_tree_shape.
-    now rewrite shape_aux.
-  Qed.
+    Lemma serialize_deserialize_shape_id :
+      forall t bytes,
+        Reader.unwrap deserialize_tree_shape
+                      (Writer.unwrap (serialize_tree_shape t) ++ bytes)
+        = Some (shape t, bytes).
+    Proof.
+      intros.
+      unfold deserialize_tree_shape.
+      now rewrite shape_aux.
+    Qed.
 
-  Fixpoint serialize_tree_elements (t : tree A) : Serializer.t :=
-    let fix serialize_tree_elements_list (l : list (tree A)) : Serializer.t :=
-        match l with
-        | [] => Serializer.empty
-        | t :: l' => Serializer.append (serialize_tree_elements t)
-                                      (serialize_tree_elements_list l')
-        end
-    in match t with
-       | atom a => serialize a
-       | node l => serialize_tree_elements_list l
-       end.
+    Fixpoint serialize_tree_elements (t : tree A) : Writer.t :=
+      let fix serialize_tree_elements_list (l : list (tree A)) : Writer.t :=
+          match l with
+          | [] => Writer.empty
+          | t :: l' => Writer.append (fun _ => (serialize_tree_elements t))
+                                     (fun _ => (serialize_tree_elements_list l'))
+          end
+      in match t with
+         | atom a => serialize a
+         | node l => serialize_tree_elements_list l
+         end.
 
-  Definition serialize_tree_elements_list :=
-    fix serialize_tree_elements_list (l : list (tree A)) : Serializer.t :=
+    Definition serialize_tree_elements_list :=
+      fix serialize_tree_elements_list (l : list (tree A)) : Writer.t :=
         match l with
-        | [] => Serializer.empty
-        | t :: l' => Serializer.append (serialize_tree_elements t)
-                                      (serialize_tree_elements_list l')
+        | [] => Writer.empty
+        | t :: l' => Writer.append (fun _ => (serialize_tree_elements t))
+                                   (fun _ => (serialize_tree_elements_list l'))
         end.
 
-  Fixpoint deserialize_tree_elements (t : tree unit) : Deserializer.t (tree A) :=
-    let fix deserialize_tree_elements_list (l : list (tree unit)) : Deserializer.t (list (tree A)) :=
-        match l with
-        | [] => Deserializer.ret []
-        | t :: l' => cons <$> deserialize_tree_elements t <*> deserialize_tree_elements_list l'
-        end
-    in match t with
-       | atom tt => @atom _ <$> deserialize
-       | node l => @node _ <$> deserialize_tree_elements_list l
-       end.
+    Fixpoint deserialize_tree_elements (t : tree unit) : Reader.t (tree A) :=
+      let fix deserialize_tree_elements_list (l : list (tree unit)) : Reader.t (list (tree A)) :=
+          match l with
+          | [] => Reader.ret []
+          | t :: l' => cons <$> deserialize_tree_elements t <*> deserialize_tree_elements_list l'
+          end
+      in match t with
+         | atom tt => @atom _ <$> deserialize
+         | node l => @node _ <$> deserialize_tree_elements_list l
+         end.
 
-  Definition deserialize_tree_elements_list :=
-    fix deserialize_tree_elements_list (l : list (tree unit)) : Deserializer.t (list (tree A)) :=
+    Definition deserialize_tree_elements_list :=
+      fix deserialize_tree_elements_list (l : list (tree unit)) : Reader.t (list (tree A)) :=
         match l with
-        | [] => Deserializer.ret []
+        | [] => Reader.ret []
         | t :: l' => cons <$> deserialize_tree_elements t <*> deserialize_tree_elements_list l'
         end.
 
-  Lemma serialize_deserialize_tree_elements_id :
-    forall t bytes,
-      Deserializer.unwrap (deserialize_tree_elements (shape t))
-                          (Serializer.unwrap (serialize_tree_elements t) ++ bytes) =
-      Some (t, bytes).
-  Proof.
-    induction t using tree_rect with
-        (P_list := fun l => forall bytes,
-           Deserializer.unwrap (deserialize_tree_elements_list (List.map shape l))
-             (Serializer.unwrap (serialize_tree_elements_list l) ++ bytes) =
-           Some (l, bytes));
-    intros;
-    cbn [shape map List.map
-         serialize_tree_shape deserialize_tree_shape
-         serialize_tree_elements deserialize_tree_elements
-         serialize_tree_elements_list deserialize_tree_elements_list].
-    - now cheerios_crush.
-    - cheerios_crush.
-      rewrite IHt.
-      cheerios_crush.
-      rewrite IHt0.
-      cheerios_crush.
-    - now cheerios_crush.
-    - fold deserialize_tree_elements_list.
-      fold serialize_tree_elements_list.
-      cheerios_crush.
-      now rewrite IHt.
-  Qed.
+    Lemma serialize_deserialize_tree_elements_id :
+      forall t bytes,
+        Reader.unwrap (deserialize_tree_elements (shape t))
+                      (Writer.unwrap (serialize_tree_elements t) ++ bytes) =
+        Some (t, bytes).
+    Proof.
+      induction t using tree_rect with
+          (P_list := fun l => forall bytes,
+                         Reader.unwrap (deserialize_tree_elements_list (List.map shape l))
+                                       (Writer.unwrap (serialize_tree_elements_list l) ++ bytes) =
+                         Some (l, bytes));
+        intros;
+        cbn [shape map List.map
+                   serialize_tree_shape deserialize_tree_shape
+                   serialize_tree_elements deserialize_tree_elements
+                   serialize_tree_elements_list deserialize_tree_elements_list].
+      - now cheerios_crush.
+      - cheerios_crush.
+        rewrite IHt.
+        cheerios_crush.
+        rewrite IHt0.
+        cheerios_crush.
+      - now cheerios_crush.
+      - fold deserialize_tree_elements_list.
+        fold serialize_tree_elements_list.
+        cheerios_crush.
+        now rewrite IHt.
+    Qed.
 
-  (* Now we serialize the tree itself by first serializing the shape, and then a
+    (* Now we serialize the tree itself by first serializing the shape, and then a
      preorder traversal of the elements. *)
-  Definition tree_serialize (t : tree A) : Serializer.t :=
-    Serializer.append (serialize_tree_shape t)
-                      (serialize_tree_elements t).
+    Definition tree_serialize (t : tree A) : Writer.t :=
+      Writer.append (fun _ => (serialize_tree_shape t))
+                    (fun _ => (serialize_tree_elements t)).
 
-  Definition tree_serialize' (t : tree A) : Serializer.t :=
-    Serializer.append (serialize_tree_shape' t)
-                      (serialize_tree_elements t).
+    Definition tree_serialize' (t : tree A) : Writer.t :=
+      Writer.append (fun _ => (serialize_tree_shape' t))
+                    (fun _ => (serialize_tree_elements t)).
 
-  (* To deserialize, we deserialize the shape and the elements, and then fill out
+    (* To deserialize, we deserialize the shape and the elements, and then fill out
      the shape with the elements. *)
-  Definition tree_deserialize : Deserializer.t (tree A) :=
-    shape <- deserialize_tree_shape ;;
-    deserialize_tree_elements shape.
+    Definition tree_deserialize : Reader.t (tree A) :=
+      shape <- deserialize_tree_shape ;;
+            deserialize_tree_elements shape.
 
-  (* To prove this correct, we need to know that serializ-/deserializing the shape of `t`
+    (* To prove this correct, we need to know that serializ-/deserializing the shape of `t`
      results in `shape t` (`serialize_deserialize_shape_id`), and that
      filling out a `map f t` with the elements of `preorder t` results in `t`
      (`fill_preorder`).
-   *)
-  Lemma tree_serialize_deserialize_id :
-    serialize_deserialize_id_spec tree_serialize tree_deserialize.
-  Proof.
-    unfold tree_serialize, tree_deserialize. cheerios_crush.
-    rewrite serialize_deserialize_shape_id.
-    now rewrite serialize_deserialize_tree_elements_id.
-  Qed.
-
-  Global Instance tree_Serializer : Serializer (tree A) :=
-    {| serialize := tree_serialize;
-        deserialize := tree_deserialize;
-        serialize_deserialize_id := tree_serialize_deserialize_id
-    |}.
-End serializer.
-
-Module sexp.
-  Import String.
-
-  Definition sexp := tree string.
-
-  Module examples.
-    (*
-       (define (id x) x)
-    *)
-    Definition id : sexp :=
-      node [atom "define"; node [atom "id"; atom "x"]; atom "x"]%string.
-
-    Lemma foo:
-           Deserializer.unwrap deserialize
-                               (Serializer.unwrap (serialize id)) = Some (id, []).
+     *)
+    Lemma tree_serialize_deserialize_id :
+      serialize_deserialize_id_spec tree_serialize tree_deserialize.
     Proof.
-      now rewrite serialize_deserialize_id_nil.
+      unfold tree_serialize, tree_deserialize. cheerios_crush.
+      rewrite serialize_deserialize_shape_id.
+      now rewrite serialize_deserialize_tree_elements_id.
     Qed.
-    (*
+
+    Global Instance tree_Serializer : Serializer (tree A) :=
+      {| serialize := tree_serialize;
+         deserialize := tree_deserialize;
+         serialize_deserialize_id := tree_serialize_deserialize_id
+      |}.
+  End serializer.
+
+  Module sexp.
+    Import String.
+
+    Definition sexp := tree string.
+
+    Module examples.
+      (*
+       (define (id x) x)
+       *)
+      Definition id : sexp :=
+        node [atom "define"; node [atom "id"; atom "x"]; atom "x"]%string.
+
+      Lemma foo:
+        Reader.unwrap deserialize
+                      (Writer.unwrap (serialize id)) = Some (id, []).
+      Proof.
+        now rewrite serialize_deserialize_id_nil.
+      Qed.
+      (*
        (define (Y f) ((lambda (x) (f (x x)))
                       (lambda (x) (f (x x)))))
-    *)
-    Definition Y : sexp :=
-      node [atom "define"; node [atom "Y"; atom "f"];
-          node [node [atom "lambda"; node [atom "x"]; node [atom "f"; node [atom "x"; atom "x"]]];
-                node [atom "lambda"; node [atom "x"]; node [atom "f"; node [atom "x"; atom "x"]]]]]
-           %string.
+       *)
+      Definition Y : sexp :=
+        node [atom "define"; node [atom "Y"; atom "f"];
+                node [node [atom "lambda"; node [atom "x"]; node [atom "f"; node [atom "x"; atom "x"]]];
+                        node [atom "lambda"; node [atom "x"]; node [atom "f"; node [atom "x"; atom "x"]]]]]
+             %string.
 
-    Lemma foo' : Deserializer.unwrap deserialize (Serializer.unwrap (serialize Y)) = Some (Y, []).
-    Proof.
-      now rewrite serialize_deserialize_id_nil.
-    Qed.
-  End examples.
-End sexp.
+      Lemma foo' : Reader.unwrap deserialize (Writer.unwrap (serialize Y)) = Some (Y, []).
+      Proof.
+        now rewrite serialize_deserialize_id_nil.
+      Qed.
+    End examples.
+  End sexp.
 
-Module JSON.
-  Module json.
-    Inductive t :=
-    | Null : t
-    | Num : nat -> t
-    | Arr : list t -> t
-    | Obj : list (String.string * t) -> t.
+  Module JSON.
+    Module json.
+      Inductive t :=
+      | Null : t
+      | Num : nat -> t
+      | Arr : list t -> t
+      | Obj : list (String.string * t) -> t.
 
-    Section json_rect.
-      Variable P : t -> Type.
+      Section json_rect.
+        Variable P : t -> Type.
 
-      Variable P_list : list t -> Type.
-      Variable P_list' : list (String.string * t) -> Type.
+        Variable P_list : list t -> Type.
+        Variable P_list' : list (String.string * t) -> Type.
 
-      Hypothesis P_nil : P_list [].
-      Hypothesis P_cons : forall j l, P j -> P_list l -> P_list (j :: l).
+        Hypothesis P_nil : P_list [].
+        Hypothesis P_cons : forall j l, P j -> P_list l -> P_list (j :: l).
 
-      Hypothesis P_nil' : P_list' [].
-      Hypothesis P_cons' : forall s j l, P j -> P_list' l -> P_list' ((s, j) :: l).
+        Hypothesis P_nil' : P_list' [].
+        Hypothesis P_cons' : forall s j l, P j -> P_list' l -> P_list' ((s, j) :: l).
 
-      Hypothesis P_null : P Null.
-      Hypothesis P_num : forall n, P (Num n).
-      Hypothesis P_arr : forall l, P_list l -> P (Arr l).
-      Hypothesis P_obj : forall l, P_list' l -> P (Obj l).
+        Hypothesis P_null : P Null.
+        Hypothesis P_num : forall n, P (Num n).
+        Hypothesis P_arr : forall l, P_list l -> P (Arr l).
+        Hypothesis P_obj : forall l, P_list' l -> P (Obj l).
 
-      Fixpoint json_rect (j : t) : P j :=
-        let fix go_list (l : list t) : P_list l :=
+        Fixpoint json_rect (j : t) : P j :=
+          let fix go_list (l : list t) : P_list l :=
+              match l with
+              | [] => P_nil
+              | j :: l => P_cons (json_rect j) (go_list l)
+              end in
+          let fix go_list' (l : list (String.string * t)) : P_list' l :=
+              match l with
+              | [] => P_nil'
+              | (s, j) :: l => P_cons' s (json_rect j) (go_list' l)
+              end in
+          match j with
+          | Null => P_null
+          | Num n => P_num n
+          | Arr l => P_arr (go_list l)
+          | Obj l => P_obj (go_list' l)
+          end.
+      End json_rect.
+
+      (* Setting P_list := List.Forall P is a reasonable default. *)
+      Check json_rect.
+      Section json_ind.
+        Variable P : t -> Prop.
+
+        Hypothesis P_null : P Null.
+        Hypothesis P_num : forall n, P (Num n).
+        Hypothesis P_arr : forall l, List.Forall P l -> P (Arr l).
+        Hypothesis P_obj : forall l, List.Forall (fun s => P (snd s)) l -> P (Obj l).
+
+        Check (fun t l Pt Pl => List.Forall_cons t Pt Pl).
+        Definition json_ind (j : t) : P j :=
+          json_rect P (List.Forall P)
+                    (List.Forall (fun s => P (snd s)))
+                    (List.Forall_nil _) (fun j l Pt Pl => List.Forall_cons j Pt Pl)
+                    (List.Forall_nil _)
+                    (fun s j l Pj Pt => List.Forall_cons (s, j) Pj Pt)
+                    P_null
+                    P_num
+                    P_arr
+                    P_obj
+                    j.
+      End json_ind.
+    End json.
+
+    Module tag.
+      Inductive t :=
+      | Null : t
+      | Num : nat -> t
+      | Str : String.string -> t
+      | Arr : t
+      | Obj : t.
+
+      (* tag serializer *)
+      Definition tag_serialize (t : t) : Writer.t :=
+        match t with
+        | Null => serialize x00
+        | Num n => Writer.append (fun _ => (serialize x01))
+                                 (fun _ => (serialize n))
+        | Str s => Writer.append (fun _ => (serialize x02))
+                                 (fun _ => (serialize s))
+        | Arr => serialize x03
+        | Obj => serialize x04
+        end.
+
+      Definition tag_deserialize : Reader.t t :=
+        tag <- deserialize ;;
+            match tag with
+            | x00 => Reader.ret Null
+            | x01 => Num <$> deserialize
+            | x02 => Str <$> deserialize
+            | x03 => Reader.ret Arr
+            | x04 => Reader.ret Obj
+            | _ => Reader.error
+            end.
+
+      Lemma tag_serialize_deserialize_id :
+        serialize_deserialize_id_spec tag_serialize tag_deserialize.
+      Proof.
+        intros.
+        destruct a;
+          unfold tag_serialize, tag_deserialize;
+          cheerios_crush; simpl; cheerios_crush.
+      Qed.
+
+      Instance tag_Serializer : Serializer t.
+      Proof.
+        exact {| serialize := tag_serialize;
+                 deserialize := tag_deserialize;
+                 serialize_deserialize_id := tag_serialize_deserialize_id |}.
+      Qed.
+      (* json <-> tree tag conversion *)
+
+      Fixpoint json_treeify (j : json.t) : tree tag.t :=
+        let fix obj_list_to_tree_list (l : list (String.string * json.t)) : list (tree tag.t) :=
             match l with
-            | [] => P_nil
-            | j :: l => P_cons (json_rect j) (go_list l)
-            end in
-        let fix go_list' (l : list (String.string * t)) : P_list' l :=
-            match l with
-            | [] => P_nil'
-            | (s, j) :: l => P_cons' s (json_rect j) (go_list' l)
-            end in
+            | [] => []
+            | (s, j) :: l => atom (tag.Str s) :: json_treeify j :: obj_list_to_tree_list l
+            end
+        in
         match j with
-        | Null => P_null
-        | Num n => P_num n
-        | Arr l => P_arr (go_list l)
-        | Obj l => P_obj (go_list' l)
+        | json.Null => atom tag.Null
+        | json.Num n => atom (tag.Num n)
+        | json.Arr l => node (atom tag.Arr :: List.map json_treeify l)
+        | json.Obj l => node (atom tag.Obj :: obj_list_to_tree_list l)
         end.
-    End json_rect.
 
-    (* Setting P_list := List.Forall P is a reasonable default. *)
-    Check json_rect.
-    Section json_ind.
-      Variable P : t -> Prop.
-
-      Hypothesis P_null : P Null.
-      Hypothesis P_num : forall n, P (Num n).
-      Hypothesis P_arr : forall l, List.Forall P l -> P (Arr l).
-      Hypothesis P_obj : forall l, List.Forall (fun s => P (snd s)) l -> P (Obj l).
-
-      Check (fun t l Pt Pl => List.Forall_cons t Pt Pl).
-      Definition json_ind (j : t) : P j :=
-        json_rect P (List.Forall P)
-                  (List.Forall (fun s => P (snd s)))
-                  (List.Forall_nil _) (fun j l Pt Pl => List.Forall_cons j Pt Pl)
-                  (List.Forall_nil _)
-                  (fun s j l Pj Pt => List.Forall_cons (s, j) Pj Pt)
-                  P_null
-                  P_num
-                  P_arr
-                  P_obj
-                  j.
-    End json_ind.
-  End json.
-
-  Module tag.
-    Inductive t :=
-    | Null : t
-    | Num : nat -> t
-    | Str : String.string -> t
-    | Arr : t
-    | Obj : t.
-
-    (* tag serializer *)
-    Definition tag_serialize (t : t) : Serializer.t :=
-      match t with
-      | Null => serialize x00
-      | Num n => Serializer.append (serialize x01) (serialize n)
-      | Str s => Serializer.append (serialize x02) (serialize s)
-      | Arr => serialize x03
-      | Obj => serialize x04
-      end.
-
-    Definition tag_deserialize : Deserializer.t t :=
-      tag <- deserialize ;;
-          match tag with
-          | x00 => Deserializer.ret Null
-          | x01 => Num <$> deserialize
-          | x02 => Str <$> deserialize
-          | x03 => Deserializer.ret Arr
-          | x04 => Deserializer.ret Obj
-          | _ => Deserializer.error
-          end.
-
-    Lemma tag_serialize_deserialize_id :
-      serialize_deserialize_id_spec tag_serialize tag_deserialize.
-    Proof.
-      intros.
-      destruct a;
-        unfold tag_serialize, tag_deserialize;
-        cheerios_crush; simpl; cheerios_crush.
-    Qed.
-
-    Instance tag_Serializer : Serializer t.
-    Proof.
-      exact {| serialize := tag_serialize;
-               deserialize := tag_deserialize;
-               serialize_deserialize_id := tag_serialize_deserialize_id |}.
-    Qed.
-    (* json <-> tree tag conversion *)
-
-    Fixpoint json_treeify (j : json.t) : tree tag.t :=
-      let fix obj_list_to_tree_list (l : list (String.string * json.t)) : list (tree tag.t) :=
-          match l with
-          | [] => []
-          | (s, j) :: l => atom (tag.Str s) :: json_treeify j :: obj_list_to_tree_list l
-          end
-      in
-      match j with
-      | json.Null => atom tag.Null
-      | json.Num n => atom (tag.Num n)
-      | json.Arr l => node (atom tag.Arr :: List.map json_treeify l)
-      | json.Obj l => node (atom tag.Obj :: obj_list_to_tree_list l)
-      end.
-
-    Definition obj_list_to_tree_list :=
-      fix obj_list_to_tree_list (l : list (String.string * json.t)) :
-        list (tree tag.t) :=
+      Definition obj_list_to_tree_list :=
+        fix obj_list_to_tree_list (l : list (String.string * json.t)) :
+          list (tree tag.t) :=
           match l with
           | [] => []
           | (s, j) :: l => atom (tag.Str s) :: json_treeify j :: obj_list_to_tree_list l
           end.
 
-    Fixpoint json_untreeify (t : tree tag.t) : option json.t :=
-      let fix untreeify_list (l : list (tree tag.t)) : option (list json.t) :=
-          match l with
-          | [] => Some []
-          | x :: l => match json_untreeify x with
-                      | None => None
-                      | Some y => match untreeify_list l with
-                                  | None => None
-                                  | Some l => Some (y :: l)
-                                  end
-                      end
-          end in
-      let fix untreeify_obj_list (l : list (tree tag.t)) :
-            option (list (String.string * json.t)) :=
-          match l with
-          | [] => Some []
-          | atom (tag.Str s) :: t :: l => match json_untreeify t with
-                           | None => None
-                           | Some j => match untreeify_obj_list l with
-                                       | None => None
-                                       | Some l => Some ((s, j) :: l)
-                                       end
-                                     end
-          | _ => None
-          end in
-      match t with
-      | atom (tag.Num n) => Some (json.Num n)
-      | node (atom tag.Arr :: l) => match untreeify_list l with
+      Fixpoint json_untreeify (t : tree tag.t) : option json.t :=
+        let fix untreeify_list (l : list (tree tag.t)) : option (list json.t) :=
+            match l with
+            | [] => Some []
+            | x :: l => match json_untreeify x with
+                        | None => None
+                        | Some y => match untreeify_list l with
                                     | None => None
-                                    | Some l => Some (json.Arr l)
+                                    | Some l => Some (y :: l)
                                     end
-      | atom (tag.Null) => Some (json.Null)
-      | node (atom tag.Obj :: l) => match untreeify_obj_list l with
-                                    | None => None
-                                    | Some l => Some (json.Obj l)
-                                    end
-      | _ => None
-      end.
+                        end
+            end in
+        let fix untreeify_obj_list (l : list (tree tag.t)) :
+              option (list (String.string * json.t)) :=
+            match l with
+            | [] => Some []
+            | atom (tag.Str s) :: t :: l => match json_untreeify t with
+                                            | None => None
+                                            | Some j => match untreeify_obj_list l with
+                                                        | None => None
+                                                        | Some l => Some ((s, j) :: l)
+                                                        end
+                                            end
+            | _ => None
+            end in
+        match t with
+        | atom (tag.Num n) => Some (json.Num n)
+        | node (atom tag.Arr :: l) => match untreeify_list l with
+                                      | None => None
+                                      | Some l => Some (json.Arr l)
+                                      end
+        | atom (tag.Null) => Some (json.Null)
+        | node (atom tag.Obj :: l) => match untreeify_obj_list l with
+                                      | None => None
+                                      | Some l => Some (json.Obj l)
+                                      end
+        | _ => None
+        end.
 
-    Definition untreeify_obj_list :=
-      fix untreeify_obj_list (l : list (tree tag.t)) :
-            option (list (String.string * json.t)) :=
+      Definition untreeify_obj_list :=
+        fix untreeify_obj_list (l : list (tree tag.t)) :
+          option (list (String.string * json.t)) :=
           match l with
           | [] => Some []
           | atom (tag.Str s) :: t :: l => match json_untreeify t with
-                           | None => None
-                           | Some j => match untreeify_obj_list l with
-                                       | None => None
-                                       | Some l => Some ((s, j) :: l)
-                                       end
-                                     end
+                                          | None => None
+                                          | Some j => match untreeify_obj_list l with
+                                                      | None => None
+                                                      | Some l => Some ((s, j) :: l)
+                                                      end
+                                          end
           | _ => None
           end.
 
-    Definition untreeify_list :=
-      fix untreeify_list l : option (list json.t) :=
+      Definition untreeify_list :=
+        fix untreeify_list l : option (list json.t) :=
           match l with
           | [] => Some []
           | x :: l => match json_untreeify x with
@@ -751,200 +778,201 @@ Module JSON.
                       end
           end.
 
-    Definition treeify_untreeify_aux (j : json.t) :=
-      json_untreeify (json_treeify j) = Some j.
+      Definition treeify_untreeify_aux (j : json.t) :=
+        json_untreeify (json_treeify j) = Some j.
 
-    Lemma treeify_untreeify_id : forall j : json.t,
-        treeify_untreeify_aux j .
-    Proof.
-      induction j using json.json_rect         with (P_list := fun l =>
-                          untreeify_list (List.map json_treeify l) = Some l)
-             (P_list' := fun l =>
-                           untreeify_obj_list (obj_list_to_tree_list l) = Some l);
-        unfold treeify_untreeify_aux;
-        auto;
-        simpl;
-        try (fold untreeify_list);
-        try (fold untreeify_obj_list);
-        try (fold obj_list_to_tree_list);
-        try (rewrite IHj);
-        try (rewrite IHj0);
-        auto.
-    Qed.
+      Lemma treeify_untreeify_id : forall j : json.t,
+          treeify_untreeify_aux j .
+      Proof.
+        induction j using json.json_rect         with (P_list := fun l =>
+                                                                   untreeify_list (List.map json_treeify l) = Some l)
+                                                      (P_list' := fun l =>
+                                                                    untreeify_obj_list (obj_list_to_tree_list l) = Some l);
+          unfold treeify_untreeify_aux;
+          auto;
+          simpl;
+          try (fold untreeify_list);
+          try (fold untreeify_obj_list);
+          try (fold obj_list_to_tree_list);
+          try (rewrite IHj);
+          try (rewrite IHj0);
+          auto.
+      Qed.
 
-    Definition json_serialize (j : json.t) :=
-      serialize (json_treeify j).
+      Definition json_serialize (j : json.t) :=
+        serialize (json_treeify j).
 
-    Definition json_deserialize : Deserializer.t json.t :=
-      j <- deserialize;;
-        match json_untreeify j with
-        | Some j => Deserializer.ret j
-        | None => Deserializer.error
-        end.
+      Definition json_deserialize : Reader.t json.t :=
+        j <- deserialize;;
+          match json_untreeify j with
+          | Some j => Reader.ret j
+          | None => Reader.error
+          end.
 
-    Lemma json_serialize_deserialize_id :
-      serialize_deserialize_id_spec json_serialize json_deserialize.
+      Lemma json_serialize_deserialize_id :
+        serialize_deserialize_id_spec json_serialize json_deserialize.
+      Proof.
+        intros.
+        unfold json_serialize, json_deserialize.
+        cheerios_crush.
+        rewrite treeify_untreeify_id.
+        cheerios_crush.
+      Qed.
+
+      Instance json_Serializer : Serializer json.t.
+      Proof.
+        exact {| serialize := json_serialize;
+                 deserialize := json_deserialize;
+                 serialize_deserialize_id := json_serialize_deserialize_id |}.
+      Qed.
+    End tag.
+
+    Definition string_eqb s s' :=
+      if (String.string_dec s s') then true else false.
+
+    Lemma string_eqb_true : forall s s', string_eqb s s' = true -> s = s'.
     Proof.
       intros.
-      unfold json_serialize, json_deserialize.
-      cheerios_crush.
-      rewrite treeify_untreeify_id.
-      cheerios_crush.
-    Qed.
-
-    Instance json_Serializer : Serializer json.t.
-    Proof.
-      exact {| serialize := json_serialize;
-               deserialize := json_deserialize;
-               serialize_deserialize_id := json_serialize_deserialize_id |}.
-    Qed.
-  End tag.
-
-  Definition string_eqb s s' :=
-    if (String.string_dec s s') then true else false.
-
-  Lemma string_eqb_true : forall s s', string_eqb s s' = true -> s = s'.
-  Proof.
-    intros.
-    unfold string_eqb in H.
-    destruct (String.string_dec s s').
-    + assumption.
-    + congruence.
-  Qed.
-
-  Lemma string_eqb_refl : forall s, string_eqb s s = true.
-  Proof.
-    intros.
-    unfold string_eqb.
-    destruct (String.string_dec s s); congruence.
-  Qed.
-
-  Fixpoint json_eqb (j j' : json.t) : bool :=
-    let fix loop_arr (l l': list json.t) : bool :=
-        match (l, l') with
-        | ([], []) => true
-        | (j :: l, j' :: l') => andb (json_eqb j j') (loop_arr l l')
-        | (_, _) => false
-        end in
-    let fix loop_obj (l l' : list (String.string * json.t)) : bool :=
-        match (l, l') with
-        | ([], []) => true
-        | ((s, j) :: l, (s', j') :: l') => andb (string_eqb s s')
-                                                (andb (json_eqb j j') (loop_obj l l'))
-        | (_, _) => false
-        end in
-    match (j, j') with
-    | (json.Null, json.Null) => true
-    | (json.Num n, json.Num n') => Nat.eqb n n'
-    | (json.Arr l, json.Arr l') => loop_arr l l'
-    | (json.Obj l, json.Obj l') => loop_obj l l'
-    | _ => false
-    end.
-  Definition loop_arr :=
-    fix loop_arr (l l': list json.t) : bool :=
-        match (l, l') with
-        | ([], []) => true
-        | (j :: l, j' :: l') => andb (json_eqb j j') (loop_arr l l')
-        | (_, _) => false
-        end.
-  Definition loop_obj :=
-    fix loop_obj (l l' : list (String.string * json.t)) : bool :=
-        match (l, l') with
-        | ([], []) => true
-        | ((s, j) :: l, (s', j') :: l') => andb (string_eqb s s')
-                                                (andb (json_eqb j j') (loop_obj l l'))
-        | (_, _) => false
-        end.
-
-  Lemma json_eqb_eq : forall j j', json_eqb j j' = true -> j = j'.
-  Proof.
-
-    induction j using json.json_rect with (P_list := fun l =>
-                                                       forall l', loop_arr l l' = true -> l = l')
-                                          (P_list' := fun l =>
-                                                        forall l', loop_obj l l' = true -> l = l');
-      unfold json_eqb.
-    - intros.
-      destruct l'.
-      + reflexivity.
-      + simpl in H. congruence.
-    - intros.
-      destruct l'.
-      + simpl in H. congruence.
-      + simpl in H.
-        apply Bool.andb_true_iff in H.
-        assert (j = t).
-        * apply IHj. apply H.
-        * assert (l = l').
-          -- apply IHj0. apply H.
-          -- now rewrite H0, H1.
-    - intros.
-      destruct l'.
-      * reflexivity.
-      * simpl in H. congruence.
-    - intros.
-      destruct l'; simpl in H.
+      unfold string_eqb in H.
+      destruct (String.string_dec s s').
+      + assumption.
       + congruence.
-      + destruct p.
-        apply Bool.andb_true_iff in H. destruct H.
-        apply Bool.andb_true_iff in H0. destruct H0.
-        assert (s = s0). now apply string_eqb_true in H.
-        assert (j = t). apply (IHj t H0).
-        assert (l = l'). apply (IHj0 _ H1).
-        now rewrite H2, H3, H4.
-    - destruct j'; try congruence.
-    - destruct j'; try congruence.
-      intros.
-      apply EqNat.beq_nat_true in H.
-      congruence.
-    - fold json_eqb.
-      fold loop_arr.
-      destruct j'; try congruence.
-      intros.
-      apply IHj in H.
-      now rewrite H.
-    - fold json_eqb.
-      fold loop_obj.
-      destruct j'; try congruence.
-      intros.
-      apply IHj in H.
-      now rewrite H.
-  Qed.
+    Qed.
 
-  Lemma json_eq_eqb : forall j j', j = j' -> json_eqb j j' = true.
-  Proof.
-    induction j using json.json_rect with (P_list := fun l => loop_arr l l = true)
-                                          (P_list' := fun l => loop_obj l l = true).
-    - reflexivity.
-    - simpl.
-      specialize IHj with j.
-      rewrite IHj0.
-      rewrite IHj; reflexivity.
-    - reflexivity.
-    - simpl.
-      rewrite string_eqb_refl, IHj0.
-      rewrite IHj; auto.      
-    - intros. now rewrite <- H.
-    - intros.  rewrite <- H. simpl.
-      symmetry.
-      apply EqNat.beq_nat_refl.
-    - intros.
-      rewrite <- H.
-      simpl.
-      assumption.
-    - intros.
-      rewrite <- H.
-      simpl.
-      assumption.
-  Qed.
+    Lemma string_eqb_refl : forall s, string_eqb s s = true.
+    Proof.
+      intros.
+      unfold string_eqb.
+      destruct (String.string_dec s s); congruence.
+    Qed.
 
-  Lemma json_eq_dec : forall j j' : json.t, {j = j'} + {j <> j'}.
-  Proof.
-    intros.
-    destruct (json_eqb j j') eqn:H.
-    + left. now apply json_eqb_eq.
-    + right. intuition.
-      rewrite json_eq_eqb in H;
+    Fixpoint json_eqb (j j' : json.t) : bool :=
+      let fix loop_arr (l l': list json.t) : bool :=
+          match (l, l') with
+          | ([], []) => true
+          | (j :: l, j' :: l') => andb (json_eqb j j') (loop_arr l l')
+          | (_, _) => false
+          end in
+      let fix loop_obj (l l' : list (String.string * json.t)) : bool :=
+          match (l, l') with
+          | ([], []) => true
+          | ((s, j) :: l, (s', j') :: l') => andb (string_eqb s s')
+                                                  (andb (json_eqb j j') (loop_obj l l'))
+          | (_, _) => false
+          end in
+      match (j, j') with
+      | (json.Null, json.Null) => true
+      | (json.Num n, json.Num n') => Nat.eqb n n'
+      | (json.Arr l, json.Arr l') => loop_arr l l'
+      | (json.Obj l, json.Obj l') => loop_obj l l'
+      | _ => false
+      end.
+    Definition loop_arr :=
+      fix loop_arr (l l': list json.t) : bool :=
+        match (l, l') with
+        | ([], []) => true
+        | (j :: l, j' :: l') => andb (json_eqb j j') (loop_arr l l')
+        | (_, _) => false
+        end.
+    Definition loop_obj :=
+      fix loop_obj (l l' : list (String.string * json.t)) : bool :=
+        match (l, l') with
+        | ([], []) => true
+        | ((s, j) :: l, (s', j') :: l') => andb (string_eqb s s')
+                                                (andb (json_eqb j j') (loop_obj l l'))
+        | (_, _) => false
+        end.
+
+    Lemma json_eqb_eq : forall j j', json_eqb j j' = true -> j = j'.
+    Proof.
+
+      induction j using json.json_rect with (P_list := fun l =>
+                                                         forall l', loop_arr l l' = true -> l = l')
+                                            (P_list' := fun l =>
+                                                          forall l', loop_obj l l' = true -> l = l');
+        unfold json_eqb.
+      - intros.
+        destruct l'.
+        + reflexivity.
+        + simpl in H. congruence.
+      - intros.
+        destruct l'.
+        + simpl in H. congruence.
+        + simpl in H.
+          apply Bool.andb_true_iff in H.
+          assert (j = t).
+          * apply IHj. apply H.
+          * assert (l = l').
+            -- apply IHj0. apply H.
+            -- now rewrite H0, H1.
+      - intros.
+        destruct l'.
+        * reflexivity.
+        * simpl in H. congruence.
+      - intros.
+        destruct l'; simpl in H.
+        + congruence.
+        + destruct p.
+          apply Bool.andb_true_iff in H. destruct H.
+          apply Bool.andb_true_iff in H0. destruct H0.
+          assert (s = s0). now apply string_eqb_true in H.
+          assert (j = t). apply (IHj t H0).
+          assert (l = l'). apply (IHj0 _ H1).
+          now rewrite H2, H3, H4.
+      - destruct j'; try congruence.
+      - destruct j'; try congruence.
+        intros.
+        apply EqNat.beq_nat_true in H.
         congruence.
-  Qed.
-End JSON.
+      - fold json_eqb.
+        fold loop_arr.
+        destruct j'; try congruence.
+        intros.
+        apply IHj in H.
+        now rewrite H.
+      - fold json_eqb.
+        fold loop_obj.
+        destruct j'; try congruence.
+        intros.
+        apply IHj in H.
+        now rewrite H.
+    Qed.
+
+    Lemma json_eq_eqb : forall j j', j = j' -> json_eqb j j' = true.
+    Proof.
+      induction j using json.json_rect with (P_list := fun l => loop_arr l l = true)
+                                            (P_list' := fun l => loop_obj l l = true).
+      - reflexivity.
+      - simpl.
+        specialize IHj with j.
+        rewrite IHj0.
+        rewrite IHj; reflexivity.
+      - reflexivity.
+      - simpl.
+        rewrite string_eqb_refl, IHj0.
+        rewrite IHj; auto.      
+      - intros. now rewrite <- H.
+      - intros.  rewrite <- H. simpl.
+        symmetry.
+        apply EqNat.beq_nat_refl.
+      - intros.
+        rewrite <- H.
+        simpl.
+        assumption.
+      - intros.
+        rewrite <- H.
+        simpl.
+        assumption.
+    Qed.
+
+    Lemma json_eq_dec : forall j j' : json.t, {j = j'} + {j <> j'}.
+    Proof.
+      intros.
+      destruct (json_eqb j j') eqn:H.
+      + left. now apply json_eqb_eq.
+      + right. intuition.
+        rewrite json_eq_eqb in H;
+          congruence.
+    Qed.
+  End JSON.
+End TreeSerializer.
